Refinery/Term/Extrinsic/Subst/Basic.lean
@@ -1,0 +1,285 @@
+import Refinery.Term.Extrinsic.Typing
+import Refinery.Term.Extrinsic.Wk
+
+namespace Refinery
+
+namespace Term
+
+open HasQuant
+
+variable {φ : Type u} {α : Type v} {ε : Type w} [S : Signature φ α ε]
+
+inductive Deriv? : Ctx? α → Var? α → Term φ (Ty α) → Type _
+  | valid {Γ : Ctx? α} {A : Ty α} {a : Term φ (Ty α)} (D : Γ ⊢ a : A) (q : EQuant)
+    (hΓ : q ≤ quant Γ) : Deriv? Γ ⟨A, q⟩ a
+  | zero {Γ : Ctx? α} (hΓ : Γ.del) (a A) : Deriv? Γ ⟨A, 0⟩ a
+
+notation Γ "⊢?" a ":" v => Deriv? Γ v a
+
+abbrev Deriv?.erase {Γ : Ctx? α} {v : Var? α} {a : Term φ (Ty α)} (_D : Γ ⊢? a : v)
+  : (Γ.erase ⊢? a : v.erase) := .zero inferInstance _ _
+
+def Deriv?.ssplitLeft {Γ : Ctx? α} {u v w : Var? α} {a : Term φ (Ty α)}
+  : (h : u.SSplit v w) → (Γ ⊢? a : u) → (h.leftCtx Γ ⊢? a : v)
+  | .left _, D => D | .sboth _, D => D
+  | .right _, D => D.erase
+
+def Deriv?.ssplitRight {Γ : Ctx? α} {u v w : Var? α} {a : Term φ (Ty α)}
+  : (h : u.SSplit v w) → (Γ ⊢? a : u) → (h.rightCtx Γ ⊢? a : w)
+  | .left _, D => D.erase | .sboth _, D => D
+  | .right _, D => D
+
+def Deriv?.unused {Γ : Ctx? α} {v : Var? α} (hΓ : Γ.del)  (a : Term φ (Ty α)) (hv : v.unused)
+  : (Γ ⊢? a : v) := match v with | ⟨A, 0⟩ => .zero hΓ a A
+
+theorem Deriv?.copy {Γ : Ctx? α} {v : Var? α} {a : Term φ (Ty α)}
+  (D : Γ ⊢? a : v) (hv : v.used) (hc : v.copy) : Γ.copy := by cases D with
+  | valid D q hΓ =>
+    cases q using EQuant.casesZero with
+    | zero => cases hv
+    | rest q =>
+      constructor
+      rw [<-EQuant.coe_le_coe]
+      apply le_trans _ hΓ
+      simp [Var?.copy_iff] at hc
+      exact hc.q
+  | zero => cases hv
+
+theorem Deriv?.del_of_unused {Γ : Ctx? α} {v : Var? α} {a : Term φ (Ty α)}
+  (D : Γ ⊢? a : v) (hv : v.unused) : Γ.del := by cases D with
+  | valid D q hΓ => cases hv; exact ⟨hΓ⟩
+  | zero hΓ _ _ => exact hΓ
+
+theorem Deriv?.del {Γ : Ctx? α} {v : Var? α} {a : Term φ (Ty α)}
+  (D : Γ ⊢? a : v) (hv : v.del) : Γ.del := by cases D with
+  | valid D q hΓ => cases q using EQuant.casesZero with
+    | zero => exact IsAff.of_zero_le_quant hΓ
+    | rest q => exact ⟨le_trans hv.q (EQuant.coe_le_coe.mpr hΓ)⟩
+  | zero hΓ _ _ => exact hΓ
+
+def Deriv?.wk {Γ Δ : Ctx? α} (ρ : Γ.Wk Δ) {v : Var? α} {a : Term φ (Ty α)}
+  (hΓΔ : quant Δ ≤ quant Γ) : (D : Δ ⊢? a : v) → (Γ ⊢? a.ren ρ : v)
+  | .valid D q hΔ => .valid (D.wk ρ) q (le_trans hΔ (EQuant.coe_le_coe.mpr hΓΔ))
+  | .zero hΓ a A => .zero (hΓ.wk ρ) (a.ren ρ) A
+
+inductive SubstDS (φ) {α ε} [S : Signature φ α ε] : Ctx? α → Ctx? α → Type _
+  | nil {Γ} (hΓ : Γ.del) : SubstDS φ Γ .nil
+  | cons {Γ Γl Γr Δ} {v} {a : Term φ _} (hΓ : Γ.SSplit Γl Γr)
+    (σ : SubstDS φ Γl Δ) (da : Γr ⊢? a : v) : SubstDS φ Γ (Δ.cons v)
+
+def SubstDS.toSubst {Γ Δ} : SubstDS φ Γ Δ → Subst φ (Ty α)
+  | .nil _, i => .invalid
+  | .cons (a := a) .., 0 => a
+  | .cons _ σ _, i + 1 => σ.toSubst i
+
+instance SubstDS.coeSubst : CoeOut (SubstDS φ Γ Δ) (Subst φ (Ty α)) where
+  coe := SubstDS.toSubst
+
+instance SubstDS.coeFun : CoeFun (SubstDS φ Γ Δ) (λ _ => Subst φ (Ty α)) where
+  coe := SubstDS.toSubst
+
+def SubstDS.tailCtx {Γ Δ} : SubstDS φ Γ Δ → Ctx? α
+  | .nil _ => Γ
+  | .cons (Γl := Γl) .. => Γl
+
+def SubstDS.headCtx {Γ Δ} : SubstDS φ Γ Δ → Ctx? α
+  | .nil _ => Γ.erase
+  | .cons (Γr := Γr) .. => Γr
+
+def SubstDS.headSplit {Γ Δ} : (σ : SubstDS φ Γ Δ) → Γ.SSplit (σ.tailCtx) (σ.headCtx)
+  | .nil _ => Γ.erase_right
+  | .cons hΓ .. => hΓ
+
+def SubstDS.head {Γ Δ} : SubstDS φ Γ Δ → Var? α
+  | .nil _ => ⟨.unit, 0⟩
+  | .cons (v := v) .. => v
+
+def SubstDS.headD {Γ Δ} : (σ : SubstDS φ Γ Δ) → σ.headCtx ⊢? σ 0 : σ.head
+  | .nil hΓ => .zero (by simp [headCtx]) _ _
+  | .cons _ _ da => da
+
+def SubstDS.tail {Γ Δ} : (σ : SubstDS φ Γ Δ) → SubstDS φ σ.tailCtx Δ.tail
+  | .nil hΓ => .nil hΓ
+  | .cons _ σ _ => σ
+
+-- def SubstDS.at {Γ Δ : Ctx? α} {q : Quant}
+--   : (σ : SubstDS φ Γ Δ) →  (hv : Δ.At ⟨A, q⟩ n) → Γ ⊢ σ n : A
+--   | .cons hΓ σ (.valid da q h), .here d hvw => sorry
+--   | .cons hΓ σ da, .there _ _ => sorry
+
+def SubstDS.wkIn {Γ' Γ Δ} (ρ : Γ'.Wk Γ) : SubstDS φ Γ Δ → SubstDS φ Γ' Δ
+  | .nil hΓ => .nil (hΓ.wk ρ)
+  | .cons hΓ σ da =>
+    .cons (hΓ.wk' ρ) (σ.wkIn (hΓ.leftWk' ρ)) (da.wk (hΓ.rightWk' ρ) (hΓ.wkRight_quant' ρ))
+
+structure SubstSSplit
+  (φ) {α ε} [S : Signature φ α ε] (inCtx outCtx outLeft outRight : Ctx? α)
+  where
+  (inLeft inRight : Ctx? α)
+  (ssplitIn : inCtx.SSplit inLeft inRight)
+  (substLeft : SubstDS φ inLeft outLeft)
+  (substRight : SubstDS φ inRight outRight)
+
+def SubstSSplit.erase_right (Γ : Ctx? α) [hΓ : Γ.del] : SubstSSplit φ Γ .nil .nil .nil
+  := ⟨Γ, Γ.erase, Γ.erase_right, .nil hΓ, .nil inferInstance⟩
+
+def SubstSSplit.erase_left (Γ : Ctx? α) [hΓ : Γ.del] : SubstSSplit φ Γ .nil .nil .nil
+  := ⟨Γ.erase, Γ, Γ.erase_left, .nil inferInstance, .nil hΓ⟩
+
+def SubstDS.ssplit {Γ Δl Δr : Ctx? α}
+  : SubstDS φ Γ Δ → Δ.SSplit Δl Δr → SubstSSplit φ Γ Δ Δl Δr
+  | .nil hΓ, .nil => SubstSSplit.erase_left _
+  | .cons (Γr := Γr) (v := v) (a := a) hΓ σ da, .cons hΔ hlr =>
+    let s := σ.ssplit hΔ
+    match hlr with
+    | .left _ =>
+      if hv : v.used then
+        let Ξ := hΓ.c12_3_23 s.ssplitIn.comm
+        let s1_23 : Γ.SSplit s.inRight Ξ := hΓ.s12_3_1_23 s.ssplitIn.comm
+        let s23 : Ξ.SSplit s.inLeft Γr := hΓ.s12_3_23 s.ssplitIn.comm
+        ⟨Ξ, s.inRight,
+          s1_23.comm,
+          s.substLeft.cons s23 da,
+          s.substRight.cons s.inRight.erase_right (.zero inferInstance a _)⟩
+      else
+        let Ξ := hΓ.c12_3_23 s.ssplitIn
+        let s1_23 : Γ.SSplit s.inLeft Ξ := hΓ.s12_3_1_23 s.ssplitIn
+        let s23 : Ξ.SSplit s.inRight Γr := hΓ.s12_3_23 s.ssplitIn
+        ⟨s.inLeft, Ξ,
+          s1_23,
+          s.substLeft.cons s.inLeft.erase_right (.unused inferInstance a (Var?.unused_iff.mpr hv)),
+          s.substRight.cons s23 (.unused (da.del_of_unused (Var?.unused_iff.mpr hv)) a rfl)⟩
+    | .right _ =>
+      let Ξ := hΓ.c12_3_23 s.ssplitIn
+      let s1_23 : Γ.SSplit s.inLeft Ξ := hΓ.s12_3_1_23 s.ssplitIn
+      let s23 : Ξ.SSplit s.inRight Γr := hΓ.s12_3_23 s.ssplitIn
+      ⟨s.inLeft, Ξ,
+        s1_23,
+        s.substLeft.cons s.inLeft.erase_right (.zero inferInstance a _),
+        s.substRight.cons s23 da⟩
+    | .sboth h =>
+      if hv : v.used then
+        have sr := Γr.both (hΓ := da.copy hv h.copy);
+        ⟨hΓ.c12_34_13 s.ssplitIn sr, hΓ.c12_34_24 s.ssplitIn sr,
+          hΓ.s12_34_13_24 s.ssplitIn sr,
+          s.substLeft.cons (hΓ.s12_34_13 s.ssplitIn sr) da,
+          s.substRight.cons (hΓ.s12_34_24 s.ssplitIn sr) da⟩
+      else
+        let Ξ := hΓ.c12_3_23 s.ssplitIn
+        let s1_23 : Γ.SSplit s.inLeft Ξ := hΓ.s12_3_1_23 s.ssplitIn
+        let s23 : Ξ.SSplit s.inRight Γr := hΓ.s12_3_23 s.ssplitIn
+        ⟨s.inLeft, Ξ,
+          s1_23,
+          s.substLeft.cons s.inLeft.erase_right (.unused inferInstance a (Var?.unused_iff.mpr hv)),
+          s.substRight.cons s23 da⟩
+
+abbrev SubstDS.inLeft {Γ Δl Δr : Ctx? α} (σ : SubstDS φ Γ Δ) (hΔ : Δ.SSplit Δl Δr) : Ctx? α
+  := (σ.ssplit hΔ).inLeft
+
+abbrev SubstDS.inRight {Γ Δl Δr : Ctx? α} (σ : SubstDS φ Γ Δ) (hΔ : Δ.SSplit Δl Δr) : Ctx? α
+  := (σ.ssplit hΔ).inRight
+
+abbrev SubstDS.ssplitIn {Γ Δl Δr : Ctx? α} (σ : SubstDS φ Γ Δ) (hΔ : Δ.SSplit Δl Δr)
+  : Γ.SSplit (σ.inLeft hΔ) (σ.inRight hΔ) := (σ.ssplit hΔ).ssplitIn
+
+abbrev SubstDS.substLeft {Γ Δl Δr : Ctx? α} (σ : SubstDS φ Γ Δ) (hΔ : Δ.SSplit Δl Δr)
+  : SubstDS φ (σ.inLeft hΔ) Δl := (σ.ssplit hΔ).substLeft
+
+abbrev SubstDS.substRight {Γ Δl Δr : Ctx? α} (σ : SubstDS φ Γ Δ) (hΔ : Δ.SSplit Δl Δr)
+  : SubstDS φ (σ.inRight hΔ) Δr := (σ.ssplit hΔ).substRight
+
+instance SubstDS.split_del_left {Γ Δl Δr : Ctx? α} (σ : SubstDS φ Γ Δ) (hΔ : Δ.SSplit Δl Δr)
+  [hl : Δl.del] : (σ.inLeft hΔ).del := by induction σ generalizing Δl Δr with
+  | nil => cases hΔ; simp [inLeft, inLeft, ssplit, SubstSSplit.erase_left]
+  | cons hΓ _ da I =>
+    cases hΔ with | cons hΔ hvw =>
+    simp only [inLeft, ssplit, ge_iff_le]
+    have I' := I hΔ (hl := hl.tail);
+    split
+    · split
+      case isTrue hv => apply Ctx?.SSplit.c12_3_23_del (h3 := da.del hl.head)
+      case isFalse => exact I'
+    · exact I'
+    · split
+      case isTrue hv => apply Ctx?.SSplit.c12_34_13_del (h3 := da.del hl.head)
+      case isFalse => exact I'
+
+instance SubstDS.split_copy_left {Γ Δl Δr : Ctx? α} (σ : SubstDS φ Γ Δ) (hΔ : Δ.SSplit Δl Δr)
+  [hl : Δl.copy] : (σ.inLeft hΔ).copy := by induction σ generalizing Δl Δr with
+  | nil => cases hΔ; simp [inLeft, inLeft, ssplit, SubstSSplit.erase_left]
+  | cons hΓ _ da I =>
+    cases hΔ with | cons hΔ hvw =>
+    simp only [inLeft, ssplit, ge_iff_le]
+    have I' := I hΔ (hl := hl.tail);
+    split
+    · split
+      case isTrue hv => apply Ctx?.SSplit.c12_3_23_copy (h3 := da.copy hv hl.head)
+      case isFalse => exact I'
+    · exact I'
+    · split
+      case isTrue hv => apply Ctx?.SSplit.c12_34_13_copy (h3 := da.copy hv hl.head)
+      case isFalse => exact I'
+
+theorem SubstDS.del {Γ Δ : Ctx? α} (σ : SubstDS φ Γ Δ) [hΔ : Δ.del] : Γ.del
+  := by
+  generalize hΔ = hΔ
+  induction σ with
+  | nil => assumption
+  | cons hΓ _ da hl =>
+    have hΓl := hl hΔ.tail
+    have hΓr := da.del hΔ.head
+    apply hΓ.in_del
+
+-- def SubstDS.lift {Γ Δ : Ctx? α} (σ : SubstDS φ Γ Δ) (v : Var? α)
+--   : SubstDS φ (Γ.cons v) (Δ.cons v) := sorry
+
+-- def Deriv.substTerm {Γ Δ : Ctx? α} (σ : SubstDS φ Γ Δ) {A : Ty α} {a : Term φ (Ty α)}
+--   : (Δ ⊢ a : A) → Term φ (Ty α)
+--   | .bv (n := n) hv => σ.toSubst n
+--   | .op (f := f) hf da => .op f (da.substTerm σ)
+--   | .let₁ (A := A) (B := B) hΔ da db =>
+--     let s := σ.ssplit hΔ;
+--     .let₁ (da.substTerm s.substRight) A (db.substTerm (s.substLeft.lift _))
+--   | .unit hv => .unit
+--   | .pair hΔ da db =>
+--     let s := σ.ssplit hΔ;
+--     .pair (da.substTerm s.substLeft) (db.substTerm s.substRight)
+--   | .let₂ (A := A) (B := B) hΔ da db =>
+--     let s := σ.ssplit hΔ;
+--     .let₂ (da.substTerm s.substRight) A B (db.substTerm ((s.substLeft.lift _).lift _))
+--   | .inl (A := A) (B := B) da => .inl A B (da.substTerm σ)
+--   | .inr (A := A) (B := B) db => .inr A B (db.substTerm σ)
+--   | .case (A := A) (B := B) hΔ da db dc =>
+--     let s := σ.ssplit hΔ;
+--     .case (da.substTerm s.substRight) A B (db.substTerm (s.substLeft.lift _))
+--           (dc.substTerm (s.substLeft.lift _))
+--   | .abort (A := A) da => .abort A (da.substTerm σ)
+--   | .iter (A := A) (B := B) hΔ _ _ da db =>
+--     let s := σ.ssplit hΔ;
+--     .iter (da.substTerm s.substRight) A B (db.substTerm (s.substLeft.lift _))
+
+-- def Deriv.subst {Γ Δ : Ctx? α} (σ : SubstDS φ Γ Δ) {A : Ty α} {a : Term φ (Ty α)}
+--   : (D : Δ ⊢ a : A) → (Γ ⊢ D.substTerm σ : A)
+--   | .bv hv => σ.at hv
+--   | .op hf da => .op hf (da.subst σ)
+--   | .let₁ hΔ da db =>
+--     let s := σ.ssplit hΔ;
+--     .let₁ s.ssplitIn (da.subst s.substRight) (db.subst (s.substLeft.lift _))
+--   | .unit _ => .unit σ.del
+--   | .pair hΔ da db =>
+--     let s := σ.ssplit hΔ;
+--     .pair s.ssplitIn (da.subst s.substLeft) (db.subst s.substRight)
+--   | .let₂ hΔ da db =>
+--     let s := σ.ssplit hΔ;
+--     .let₂ s.ssplitIn (da.subst s.substRight) (db.subst ((s.substLeft.lift _).lift _))
+--   | .inl da => .inl (da.subst σ)
+--   | .inr db => .inr (db.subst σ)
+--   | .case hΔ da db dc =>
+--     let s := σ.ssplit hΔ;
+--     .case s.ssplitIn (da.subst s.substRight) (db.subst (s.substLeft.lift _))
+--           (dc.subst (s.substLeft.lift _))
+--   | .abort da => .abort (da.subst σ)
+--   | .iter hΔ _ _ da db =>
+--     let s := σ.ssplit hΔ;
+--     .iter s.ssplitIn (σ.split_copy_left hΔ) (σ.split_del_left hΔ)
+--                         (da.subst s.substRight) (db.subst (s.substLeft.lift _))
